Integrate property transfer partly with motor function

src/tools/symbexec/examples/analysis/motorfunc_transfScript.sml
@@ -31,23 +31,22 @@ val birs_state_ss = rewrites (type_rws ``:birs_state_t``);
 
 val _ = new_theory "motorfunc_transf";
 
-val _ = export_theory();
-
 
 
 val bprog_def = motorfuncTheory.bprog_def;
 val bprog = (fst o dest_eq o concl) bprog_def;
+val bprog_tm = (fst o dest_eq o concl) bprog_def;
 
 
 
 
-val m0_mod_vars_def = motorfuncTheory.m0_mod_vars_def;
+val m0_mod_vars_def = bir_program_transfTheory.m0_mod_vars_def;
 
-val m0_mod_vars_thm = motorfuncTheory.m0_mod_vars_thm;
+val m0_mod_vars_thm = bir_program_transfTheory.m0_mod_vars_thm;
 
-val birenvtyl_def = motorfuncTheory.birenvtyl_def;
+val birenvtyl_def = bir_program_transfTheory.birenvtyl_def;
 
-val birenvtyl_EVAL_thm = motorfuncTheory.birenvtyl_EVAL_thm;
+val birenvtyl_EVAL_thm = bir_program_transfTheory.birenvtyl_EVAL_thm;
 
 
 
@@ -490,20 +489,15 @@ val bprog_bir_prop_thm = save_thm(
 );
 (* ........................... *)
 
-val bir_step_n_in_L_jgmt_thm = prove(``
-(bir_step_n_in_L_jgmt
-  bprog
-  <|bpc_label := BL_Address (Imm32 2824w); bpc_index := 0|>
-  motor_analysis_L
-  (\st.
-       st.bst_status = BST_Running /\
+val bir_frag_l_tm = ``<|bpc_label := BL_Address (Imm32 2824w); bpc_index := 0|>``;
+val bir_frag_l_ml_tm = (snd o dest_comb o snd o dest_comb o snd o dest_eq o concl o EVAL) ``(^bir_frag_l_tm).bpc_label``;
 
-       (* TODO: this was added *)
-       st.bst_pc.bpc_index = 0 /\
+val bir_frag_l_exit_ml_tm = ``2886w:word32``;
+val bir_frag_l_exit_tm = ``<|bpc_label := BL_Address (Imm32 ^bir_frag_l_exit_ml_tm); bpc_index := 0|>``;
 
-       bir_envty_list_b birenvtyl st.bst_environ /\
-       bir_eval_exp
-         (BExp_BinExp BIExp_And
+val bprecond_def = Define `
+    bprecond =
+         BExp_BinExp BIExp_And
             (BExp_BinExp BIExp_And
                (BExp_BinPred BIExp_LessOrEqual (BExp_Const (Imm32 0xFFFFFFw))
                   (BExp_Den (BVar "SP_process" (BType_Imm Bit32))))
@@ -511,42 +505,59 @@ val bir_step_n_in_L_jgmt_thm = prove(``
                   (BExp_Den (BVar "SP_process" (BType_Imm Bit32)))))
             (BExp_BinPred BIExp_LessOrEqual
                (BExp_Den (BVar "countw" (BType_Imm Bit64)))
-               (BExp_Const (Imm64 0xFFFFFFFFFFFFFF00w)))) st.bst_environ =
-       SOME bir_val_true)
-  (\st st'.
-         (st'.bst_pc = <|bpc_label := BL_Address (Imm32 2886w); bpc_index := 0|>) /\
+               (BExp_Const (Imm64 0xFFFFFFFFFFFFFF00w)))
+`;
 
-         (* TODO: this was added *)
-         st'.bst_status = BST_Running /\
+val pre_bir_def = Define `
+    pre_bir bs =
+       (bir_eval_exp bprecond bs.bst_environ = SOME bir_val_true)
+`;
 
-         ?v1 v2.
-           bir_env_lookup "countw" st.bst_environ =
-           SOME (BVal_Imm (Imm64 v1)) /\
-           bir_env_lookup "countw" st'.bst_environ =
-           SOME (BVal_Imm (Imm64 v2)) /\
+val post_bir_def = Define `
+    post_bir bs1 bs2 =
+      (?v1 v2. bir_env_lookup "countw" bs1.bst_environ = SOME (BVal_Imm (Imm64 v1)) /\
+               bir_env_lookup "countw" bs2.bst_environ = SOME (BVal_Imm (Imm64 v2)) /\
+               (v1 <=+ 0xFFFFFFFFFFFFFF00w) /\
+               (v1 + 44w <=+ v2) /\
+               (v2 <=+ v1 + 47w))
+(*
            v1 <+ v2 /\
            v1 + 44w <=+ v2 /\
-           v2 <=+ v1 + 47w))
+           v2 <=+ v1 + 47w
+*)
+`;
+
+val pre_bir_nL_def = Define `
+    pre_bir_nL st =
+      (
+       st.bst_status = BST_Running /\
+       st.bst_pc.bpc_index = 0 /\
+       bir_envty_list_b birenvtyl st.bst_environ /\
+
+       pre_bir st
+      )
+`;
+val post_bir_nL_def = Define `
+    post_bir_nL (st:bir_state_t) st' =
+      (
+         (st'.bst_pc = ^bir_frag_l_exit_tm) /\
+         st'.bst_status = BST_Running /\
+
+         post_bir st st'
+      )
+`;
+
+val bir_step_n_in_L_jgmt_thm = prove(``
+bir_step_n_in_L_jgmt
+  ^bprog_tm
+  ^bir_frag_l_tm
+  motor_analysis_L
+  pre_bir_nL
+  post_bir_nL
 ``,
   cheat
 );
 
-
-
-
-
-
-
-
-(*
-"bir_backlifterTheory.bir_exec_to_labels_TO_exec_to_addr_label_n"
-*)
-
-(*
-
-TODO: establish relational postcondition
-
-*)
 
 val motor_analysis_L_INTER_thm = prove(``
 motor_analysis_L INTER
@@ -568,90 +579,392 @@ motor_analysis_L INTER
   EVAL_TAC
 );
 
-val bir_abstract_jgmt_rel_thm = prove(``
-(abstract_jgmt_rel
-  (bir_etl_wm bprog)
-  (BL_Address (Imm32 2824w))
-  {BL_Address (Imm32 2886w)}
-  (\st.
-       st.bst_status = BST_Running /\
-
-       (* TODO: this was added *)
-       st.bst_pc.bpc_index = 0 /\
-
-       bir_envty_list_b birenvtyl st.bst_environ /\
-       bir_eval_exp
-         (BExp_BinExp BIExp_And
-            (BExp_BinExp BIExp_And
-               (BExp_BinPred BIExp_LessOrEqual (BExp_Const (Imm32 0xFFFFFFw))
-                  (BExp_Den (BVar "SP_process" (BType_Imm Bit32))))
-               (BExp_Aligned Bit32 2
-                  (BExp_Den (BVar "SP_process" (BType_Imm Bit32)))))
-            (BExp_BinPred BIExp_LessOrEqual
-               (BExp_Den (BVar "countw" (BType_Imm Bit64)))
-               (BExp_Const (Imm64 0xFFFFFFFFFFFFFF00w)))) st.bst_environ =
-       SOME bir_val_true)
-  (\st st'.
-         (* TODO: this was added *)
-         st'.bst_status = BST_Running /\
-
-         ?v1 v2.
-           bir_env_lookup "countw" st.bst_environ =
-           SOME (BVal_Imm (Imm64 v1)) /\
-           bir_env_lookup "countw" st'.bst_environ =
-           SOME (BVal_Imm (Imm64 v2)) /\
-           v1 <+ v2 /\
-           v1 + 44w <=+ v2 /\
-           v2 <=+ v1 + 47w))
+val bir_abstract_jgmt_rel_motor_thm = prove(``
+abstract_jgmt_rel
+  (bir_etl_wm ^bprog_tm)
+  (BL_Address (Imm32 ^bir_frag_l_ml_tm))
+  {BL_Address (Imm32 ^bir_frag_l_exit_ml_tm)}
+  pre_bir_nL
+  post_bir_nL
 ``,
   ASSUME_TAC
-    (Q.SPEC `{BL_Address (Imm32 2886w)}`
+    (Q.SPEC `{BL_Address (Imm32 ^bir_frag_l_exit_ml_tm)}`
       (MATCH_MP
         (REWRITE_RULE
            [bir_programTheory.bir_block_pc_def]
            bir_program_transfTheory.bir_step_n_in_L_jgmt_TO_abstract_jgmt_rel_thm)
         bir_step_n_in_L_jgmt_thm)) >>
 
-  FULL_SIMP_TAC std_ss [IMAGE_SING, IN_SING, bir_programTheory.bir_block_pc_def] >>
+  FULL_SIMP_TAC std_ss [pre_bir_nL_def] >>
 
+  FULL_SIMP_TAC std_ss [IMAGE_SING, IN_SING, bir_programTheory.bir_block_pc_def] >>
   FULL_SIMP_TAC (std_ss++holBACore_ss) [motor_analysis_L_INTER_thm] >>
 
-  FULL_SIMP_TAC (std_ss++holBACore_ss) [abstract_jgmt_rel_def] >>
-  METIS_TAC []
+  FULL_SIMP_TAC std_ss [post_bir_nL_def] >>
+  FULL_SIMP_TAC (std_ss++holBACore_ss) [abstract_jgmt_rel_def]
 );
+
+val bmemms_t = List.nth((snd o strip_comb o concl) bin_motor_funcTheory.bin_motor_func_thm, 2);
+val bmemms_def = Define `
+    bmemms = ^(bmemms_t)
+`;
+val bin_motor_func_thm = REWRITE_RULE [GSYM bmemms_def, GSYM bprog_def] bin_motor_funcTheory.bin_motor_func_thm;
+
+
+(* TODO: COPIED STUFF *)
+(* =================================================================================== *)
+val bmr_rel_m0_mod_bmr_IMP_index_thm = prove(``
+!ms bs.
+  (bmr_rel (m0_mod_bmr (F,T)) bs ms) ==>
+  (bs.bst_status = BST_Running) ==>
+  (bs.bst_pc.bpc_index = 0)
+``,
+  EVAL_TAC >>
+  REPEAT STRIP_TAC >> (
+    FULL_SIMP_TAC (std_ss++holBACore_ss) []
+  )
+);
+
+val bmr_rel_m0_mod_bmr_IMP_countw_lookup_thm = prove(``
+!bs ms.
+  (bmr_rel (m0_mod_bmr (F,T)) bs ms) ==>
+  (bir_env_lookup "countw" bs.bst_environ = SOME (BVal_Imm (Imm64 ms.countw)))
+``,
+  EVAL_TAC >>
+  REPEAT STRIP_TAC >> (
+    FULL_SIMP_TAC (std_ss++holBACore_ss) []
+  ) >> (
+    METIS_TAC []
+  )
+);
+
+val bmr_rel_m0_mod_bmr_IMP_SP_process_lookup_thm = prove(``
+!bs ms.
+  (bmr_rel (m0_mod_bmr (F,T)) bs ms) ==>
+  (bir_env_lookup "SP_process" bs.bst_environ = SOME (BVal_Imm (Imm32 (ms.base.REG RName_SP_process))))
+``,
+  EVAL_TAC >>
+  REPEAT STRIP_TAC >> (
+    FULL_SIMP_TAC (std_ss++holBACore_ss) []
+  ) >> (
+    METIS_TAC []
+  )
+);
+(* =================================================================================== *)
 
 (*
   transfer of relational postcondition to machine model
 *)
-val m0_mod_thm = prove(``
-(abstract_jgmt_rel
-  m0_mod_weak_model
-  (2824w)
-  {2886w}
-  (\ms.
-      (EVERY (bmr_ms_mem_contains (m0_mod_bmr (T,T)) ms) mms) /\
-      ((m0_mod_bmr (T,T)).bmr_extra ms) /\
+val pre_m0_mod_def = Define `
+    pre_m0_mod ms =
+      (
+        (EVERY (bmr_ms_mem_contains (m0_mod_bmr (F,T)) ms) bmemms) /\
+        ((m0_mod_bmr (F,T)).bmr_extra ms) /\
 
-      (0xFFFFFFw <=+ ms.base.REG RName_SP_process) /\
-      (ms.base.REG RName_SP_process && 0x3w = 0w) /\
-      (ms.countw <=+ 0xFFFFFFFFFFFFFF00w))
-  (\ms ms'.
-      ms.countw <+ ms'.countw /\
-      ms.countw + 44w <=+ ms'.countw /\
-      ms'.countw <=+ ms.countw + 47w))
+        (0xFFFFFFw <=+ ms.base.REG RName_SP_process /\
+         ms.base.REG RName_SP_process && 0x3w = 0w /\
+         ms.countw <=+ 0xFFFFFFFFFFFFFF00w)
+      )
+`;
+val post_m0_mod_def = Define `
+    post_m0_mod ms ms' =
+      (
+        (ms.countw <=+ 0xFFFFFFFFFFFFFF00w) /\
+        (ms.countw + 44w <=+ ms'.countw) /\
+        (ms'.countw <=+ ms.countw + 47w)
+      )
+`;
+
+val backlift_bir_m0_mod_pre_abstr_ex_thm = prove(``
+  backlift_bir_m0_mod_pre_abstr pre_m0_mod pre_bir_nL
+``,
+  FULL_SIMP_TAC std_ss [backlift_bir_m0_mod_pre_abstr_def, pre_m0_mod_def, pre_bir_nL_def, pre_bir_def] >>
+  REPEAT GEN_TAC >>
+  REPEAT DISCH_TAC >>
+
+  IMP_RES_TAC bmr_rel_m0_mod_bmr_IMP_index_thm >>
+  FULL_SIMP_TAC std_ss [] >>
+
+  REWRITE_TAC [bprecond_def] >>
+  EVAL_TAC >>
+
+  IMP_RES_TAC bmr_rel_m0_mod_bmr_IMP_countw_lookup_thm >>
+  IMP_RES_TAC bmr_rel_m0_mod_bmr_IMP_SP_process_lookup_thm >>
+  ASM_REWRITE_TAC [] >>
+  EVAL_TAC >>
+  ASM_REWRITE_TAC [] >>
+  EVAL_TAC
+);
+
+val backlift_bir_m0_mod_post_concr_ex_thm = prove(``
+  backlift_bir_m0_mod_post_concr post_bir_nL post_m0_mod
+``,
+  FULL_SIMP_TAC std_ss [backlift_bir_m0_mod_post_concr_def, post_bir_nL_def, post_m0_mod_def, post_bir_def] >>
+  REPEAT GEN_TAC >>
+  REPEAT DISCH_TAC >>
+  FULL_SIMP_TAC std_ss [] >>
+
+  `v1 = ms.countw` by (
+    IMP_RES_TAC bmr_rel_m0_mod_bmr_IMP_countw_lookup_thm >>
+    FULL_SIMP_TAC (std_ss++holBACore_ss) []
+  ) >>
+
+  `v2 = ms'.countw` by (
+    IMP_RES_TAC bmr_rel_m0_mod_bmr_IMP_countw_lookup_thm >>
+    FULL_SIMP_TAC (std_ss++holBACore_ss) []
+  ) >>
+
+  FULL_SIMP_TAC (std_ss) []
+);
+
+val m0_mod_thm = prove(``
+abstract_jgmt_rel
+  m0_mod_weak_model
+  (^bir_frag_l_ml_tm)
+  {^bir_frag_l_exit_ml_tm}
+  pre_m0_mod
+  post_m0_mod
 ``,
 
-  cheat
-(*
-bir_program_transfTheory.backlift_bir_m0_mod_contract_thm
-*)
+  ASSUME_TAC
+    (Q.SPECL
+      [`pre_m0_mod`, `pre_bir_nL`, `post_bir_nL`, `post_m0_mod`, `(^bir_frag_l_ml_tm)`, `{^bir_frag_l_exit_ml_tm}`]
+      (MATCH_MP
+        bir_program_transfTheory.backlift_bir_m0_mod_contract_thm
+        (bin_motor_func_thm))) >>
+
+  `!ms. pre_m0_mod ms ==>
+           EVERY (bmr_ms_mem_contains (m0_mod_bmr (F,T)) ms) bmemms` by (
+    FULL_SIMP_TAC std_ss [pre_m0_mod_def]
+  ) >>
+
+  `!ms. pre_m0_mod ms ==> (m0_mod_bmr (F,T)).bmr_extra ms` by (
+    FULL_SIMP_TAC std_ss [pre_m0_mod_def]
+  ) >>
+
+  `!bs.    pre_bir_nL bs ==>
+           ~bir_state_is_terminated bs` by (
+    FULL_SIMP_TAC std_ss [pre_bir_nL_def, bir_programTheory.bir_state_is_terminated_def]
+  ) >>
+
+  `MEM (BL_Address (Imm32 ^bir_frag_l_ml_tm)) (bir_labels_of_program (bprog:'observation_type bir_program_t))` by (
+    EVAL_TAC
+  ) >>
+  FULL_SIMP_TAC std_ss [] >>
+
+  `!bs bs'. post_bir_nL bs bs' ==> ~bir_state_is_terminated bs'` by (
+    FULL_SIMP_TAC std_ss [post_bir_nL_def, bir_programTheory.bir_state_is_terminated_def]
+  ) >>
+
+  ASSUME_TAC backlift_bir_m0_mod_pre_abstr_ex_thm >>
+  ASSUME_TAC backlift_bir_m0_mod_post_concr_ex_thm >>
+
+  FULL_SIMP_TAC std_ss [IMAGE_SING, IN_SING] >>
+  FULL_SIMP_TAC std_ss [bir_abstract_jgmt_rel_motor_thm] >>
+  METIS_TAC []
 );
 
 
+(* TODO: MORE COPIED STUFF *)
+(* =================================================================================== *)
+val m0_mod_R_IMP_bmr_ms_mem_contains_thm = prove(``
+!mms ms.
+  (m0_mod_R ms mms) ==>
+  (bmr_ms_mem_contains (m0_mod_bmr (F,T)) mms =
+   bmr_ms_mem_contains (m0_bmr (F,T)) ms)
+``,
+  REWRITE_TAC [m0_mod_R_def, m0_mod_stepTheory.m0_mod_inv_def] >>
+  REPEAT STRIP_TAC >>
+
+  MATCH_MP_TAC boolTheory.EQ_EXT >>
+  Cases_on `x` >>
+
+  `(mms.base with count := w2n mms.countw).MEM = mms.base.MEM` by (
+    SIMP_TAC (std_ss++(rewrites (type_rws ``:m0_state``))) []
+  ) >>
+
+  Q.SPEC_TAC (`q`, `b`) >>
+  Q.SPEC_TAC (`r`, `l`) >>
+
+  Induct_on `l` >- (
+    GEN_TAC >>
+    EVAL_TAC
+  ) >>
+
+  REWRITE_TAC [bir_lifting_machinesTheory.bmr_ms_mem_contains_def] >>
+  REPEAT STRIP_TAC >>
+  POP_ASSUM (fn thm => SIMP_TAC std_ss [thm]) >>
+
+  SIMP_TAC std_ss [bir_lifting_machinesTheory.bmr_mem_lf_def] >>
+
+  SIMP_TAC (std_ss++(rewrites (type_rws ``:('a,'b,'c) bir_lifting_machine_rec_t``))) [bir_lifting_machinesTheory.m0_mod_bmr_def, bir_lifting_machinesTheory.m0_bmr_def] >>
+
+  FULL_SIMP_TAC (std_ss++holBACore_ss) [bir_lifting_machinesTheory.m0_mod_lifted_mem_def, bir_lifting_machinesTheory.m0_lifted_mem_def] >>
+  CASE_TAC >>
+
+  FULL_SIMP_TAC (std_ss++holBACore_ss) [bir_lifting_machinesTheory.bir_machine_lifted_mem_t_11] >>
+  POP_ASSUM (ASSUME_TAC o GSYM) >>
+  ASM_SIMP_TAC (std_ss++holBACore_ss) []
+);
+val m0_mod_R_IMP_REG_EQ_thm = prove(``
+!mms ms.
+  (m0_mod_R ms mms) ==>
+  (mms.base.REG = ms.REG)
+``,
+  REWRITE_TAC [m0_mod_R_def, m0_mod_stepTheory.m0_mod_inv_def] >>
+  REPEAT STRIP_TAC >>
+
+  ASM_SIMP_TAC (std_ss++(rewrites (type_rws ``:m0_state``))) []
+);
+val m0_mod_R_IMP_bmr_extra_thm = prove(``
+!mms ms.
+  (m0_mod_R ms mms) ==>
+  ((m0_mod_bmr (F,T)).bmr_extra mms = (m0_bmr (F,T)).bmr_extra ms)
+``,
+  REWRITE_TAC [m0_mod_R_def, m0_mod_stepTheory.m0_mod_inv_def] >>
+  REPEAT STRIP_TAC >>
+
+  SIMP_TAC (std_ss++(rewrites (type_rws ``:('a,'b,'c) bir_lifting_machine_rec_t``))) [bir_lifting_machinesTheory.m0_mod_bmr_def, bir_lifting_machinesTheory.m0_bmr_def] >>
+  ASM_SIMP_TAC (std_ss++holBACore_ss) [bir_lifting_machinesTheory.m0_mod_state_is_OK_def, bir_lifting_machinesTheory.m0_state_is_OK_def] >>
+
+  ASM_SIMP_TAC (std_ss++(rewrites (type_rws ``:m0_state``))) []
+);
+val m0_mod_R_IMP_count_EQ_countw_thm = prove(``
+!mms ms.
+  (m0_mod_R ms mms) ==>
+  (ms.count = w2n mms.countw)
+``,
+  REWRITE_TAC [m0_mod_R_def, m0_mod_stepTheory.m0_mod_inv_def] >>
+  REPEAT STRIP_TAC >>
+
+  ASM_SIMP_TAC (std_ss++(rewrites (type_rws ``:m0_state``))) []
+);
+
+(* =================================================================================== *)
+
 (*
-TODO: transfer to (unmodified) m0 model
+transfer to (unmodified) m0 model
 *)
 
+val pre_m0_def = Define `
+    pre_m0 ms =
+      (
+        (EVERY (bmr_ms_mem_contains (m0_bmr (F,T)) ms) bmemms) /\
+        ((m0_bmr (F,T)).bmr_extra ms) /\
+
+        (0xFFFFFFw <=+ ms.REG RName_SP_process /\
+         ms.REG RName_SP_process && 0x3w = 0w /\
+         ms.count <= 0xFFFFFFFFFFFFFF00:num)
+      )
+`;
+val post_m0_def = Define `
+    post_m0 ms ms' =
+      (
+        (ms.count + 44 <= ms'.count) /\
+        (ms'.count <= ms.count + 47)
+      )
+`;
 
 
-val _ = print_term (concl bprog_bir_prop_thm);
+
+val backlift_m0_mod_m0_pre_abstr_ex_thm = prove(``
+  backlift_m0_mod_m0_pre_abstr (pre_m0) (pre_m0_mod)
+``,
+  FULL_SIMP_TAC std_ss [pre_m0_def, pre_m0_mod_def, backlift_m0_mod_m0_pre_abstr_def, backlift_m0_mod_m0_post_concr_def] >>
+
+  REPEAT GEN_TAC >>
+  REPEAT DISCH_TAC >>
+  FULL_SIMP_TAC std_ss [] >>
+
+  `(EVERY (bmr_ms_mem_contains (m0_mod_bmr (F,T)) mms) bmemms) /\
+        ((m0_mod_bmr (F,T)).bmr_extra mms)` by (
+    METIS_TAC [m0_mod_R_IMP_bmr_ms_mem_contains_thm, m0_mod_R_IMP_bmr_extra_thm]
+  ) >>
+  FULL_SIMP_TAC std_ss [] >>
+
+  `0xFFFFFFw <=+ mms.base.REG RName_SP_process /\
+   mms.base.REG RName_SP_process && 0x3w = 0w` by (
+    METIS_TAC [m0_mod_R_IMP_REG_EQ_thm]
+  ) >>
+  FULL_SIMP_TAC std_ss [] >>
+
+(*
+         ms.count <= 0xFFFFFFFFFFFFFF00:num ==>
+         ms.countw <=+ 0xFFFFFFFFFFFFFF00w
+*)
+  REWRITE_TAC [wordsTheory.WORD_LS] >>
+
+  IMP_RES_TAC m0_mod_R_IMP_count_EQ_countw_thm >>
+  POP_ASSUM (fn thm => REWRITE_TAC [GSYM thm]) >>
+  EVAL_TAC >>
+  ASM_REWRITE_TAC []
+);
+
+val backlift_m0_mod_m0_post_concr_ex_thm = prove(``
+  backlift_m0_mod_m0_post_concr post_m0_mod post_m0
+``,
+  FULL_SIMP_TAC std_ss [post_m0_mod_def, post_m0_def, backlift_m0_mod_m0_pre_abstr_def, backlift_m0_mod_m0_post_concr_def] >>
+  REPEAT GEN_TAC >>
+  REPEAT DISCH_TAC >>
+  FULL_SIMP_TAC std_ss [] >>
+
+  IMP_RES_TAC m0_mod_R_IMP_count_EQ_countw_thm >>
+  ASM_REWRITE_TAC [] >>
+
+  cheat
+(*
+  METIS_TAC [m0_mod_R_IMP_bmr_ms_mem_contains_thm, m0_mod_R_IMP_bmr_extra_thm, m0_mod_R_IMP_REG_EQ_thm]
+*)
+);
+
+val m0_thm = store_thm(
+   "m0_thm", ``
+abstract_jgmt_rel
+  m0_weak_model
+  (^bir_frag_l_ml_tm)
+  {^bir_frag_l_exit_ml_tm}
+  (pre_m0)
+  (post_m0)
+``,
+
+  ASSUME_TAC
+    (Q.SPECL
+      [`pre_m0`, `pre_m0_mod`, `post_m0_mod`, `post_m0`, `(^bir_frag_l_ml_tm)`, `{^bir_frag_l_exit_ml_tm}`]
+      bir_program_transfTheory.backlift_m0_mod_m0_contract_thm) >>
+
+  `!ms. pre_m0 ms ==> (\ms. ms.count < 2 ** 64) ms` by (
+    FULL_SIMP_TAC std_ss [pre_m0_def] >>
+    REPEAT STRIP_TAC >>
+
+(*
+    IMP_RES_TAC arithmeticTheory.LESS_EQ_IMP_LESS_SUC >>
+    POP_ASSUM (ASSUME_TAC o CONV_RULE EVAL) >>
+*)
+    IMP_RES_TAC arithmeticTheory.LESS_EQ_LESS_TRANS >>
+    POP_ASSUM MATCH_MP_TAC >>
+    EVAL_TAC
+  ) >>
+
+  ASSUME_TAC backlift_m0_mod_m0_pre_abstr_ex_thm >>
+  ASSUME_TAC backlift_m0_mod_m0_post_concr_ex_thm >>
+
+  FULL_SIMP_TAC std_ss [m0_mod_thm]
+);
+
+val m0_EVAL_thm = save_thm(
+   "m0_EVAL_thm",
+  REWRITE_RULE
+   [pre_m0_def, post_m0_def,
+    prove(``pre_m0 = (\ms. pre_m0 ms)``, MATCH_MP_TAC boolTheory.EQ_EXT >> FULL_SIMP_TAC std_ss []),
+    prove(``post_m0 = (\ms ms'. post_m0 ms ms')``, MATCH_MP_TAC boolTheory.EQ_EXT >> FULL_SIMP_TAC std_ss [] >> GEN_TAC >> MATCH_MP_TAC boolTheory.EQ_EXT >> FULL_SIMP_TAC std_ss [])]
+   m0_thm
+);
+
+val _ = export_theory();
+
+val result = m0_EVAL_thm;
+
+val _ = (print_term o concl) result;
+
+val _ = show_tags := true;
+val _ = Portable.pprint Tag.pp_tag (tag result);
